examples/compcert/experiment1/verif_exp1.v
@@ -1,5 +1,4 @@
 Require Import VST.floyd.forward.
-
 Require Import VST.floyd.proofauto. (* Import the Verifiable C system *) 
 Require Import exp1. (* Import the AST of this C program *) 
 (* The next line is "boilerplate", always required after importing an AST. *) 
@@ -7,8 +6,12 @@ Instance CompSpecs : compspecs. make_compspecs prog. Defined.
 Definition Vprog : varspecs.  mk_varspecs prog. Defined. 
 
 (* Functional spec of this program.  *)
-Definition myAdd : Z -> Z -> Z := Z.add.
 
+Definition myId (a:Z) : Z := a.
+
+Definition myAdd : Z -> Z := myId.
+
+(*
 Lemma assoc : forall a b c : Z, (a+(b+c)) = (a+b+c).
 Proof.
   intuition.
@@ -25,19 +28,19 @@ Proof.
   exists (0-a).
   intuition.
 Qed.
+*)
 
 (* Beginning of the API spec for the sumarray.c program *)
-Definition exp1_spec : ident * funspec :=
- DECLARE _mySum
-  WITH x:val, y:val, sh : share, sum : Z
-  PRE [ _x OF tint, _y OF tint ]
-          PROP  (readable_share sh;
-                 0 <= sum <= Int.max_signed)
-          LOCAL (temp _x x; temp _y y)
-          SEP   (data_at sh (tint) (Vint (Int.repr sum)) x)
+Definition myId_spec : ident * funspec :=
+ DECLARE _myId
+  WITH x:val, ret : Z
+  PRE [ _x OF tint ]
+          PROP  ( x = Vint (Int.repr ret) )
+          LOCAL (temp _x x)
+          SEP   ()
   POST [ tint ]
-        PROP () LOCAL(temp ret_temp  (Vint (Int.repr (sum))))
-           SEP (data_at sh (tint) (Vint (Int.repr sum)) x).
+        PROP () LOCAL(temp ret_temp  (Vint (Int.repr (ret))))
+           SEP ().
 
 
 (* The precondition of "int main(void){}" always looks like this. *)
@@ -47,24 +50,16 @@ Definition main_spec :=
   PRE  [] main_pre prog nil gv
   POST [ tint ]  
      PROP() 
-     LOCAL (temp ret_temp (Vint (Int.repr (2+3)))) 
+     LOCAL (temp ret_temp (Vint (Int.repr (2)))) 
      SEP(TT).
-
 
 (* Packaging the API spec all together. *)
 Definition Gprog : funspecs :=
-        ltac:(with_library prog [exp1_spec; main_spec]).
+        ltac:(with_library prog [myId_spec; main_spec]).
 
-
-(** Proof that f_sumarray, the body of the sumarray() function,
- ** satisfies sumarray_spec, in the global context (Vprog,Gprog).
- **)
-Lemma body_mySum: semax_body Vprog Gprog f_mySum exp1_spec.
+Lemma body_myId: semax_body Vprog Gprog f_myId myId_spec.
 Proof.
 start_function. (* Always do this at the beginning of a semax_body proof *)
-(* The next two lines do forward symbolic execution through
-   the first two executable statements of the function body *)
-forward.
 forward.
 Qed.
 
@@ -72,14 +67,10 @@ Lemma body_main:  semax_body Vprog Gprog f_main main_spec.
 Proof.
 start_function.
 forward.
-forward.
 forward_call (* provide a witness to the WITH clause of exp1_spec *)
-  (Vint (Int.repr 2), Vint (Int.repr 3), Ews ,5).
-Focus 2. split. auto. computable.
-Focus 2. forward.
-
-(* Not sure how to tackle this goal. *)
-Admitted.
+  (Vint (Int.repr 2), 2).
+forward.
+Qed.
 
 Existing Instance NullExtension.Espec.
 
@@ -88,15 +79,10 @@ Locate semax_func.
 Lemma prog_correct:
   semax_prog prog Vprog Gprog.
 Proof.
-prove_semax_prog. 
-Admitted. Abort.
-(*
-This proof fails here.
-It matches the example, though
-*)
-(*
-semax_func_cons body_mySum.
+prove_semax_prog.
+semax_func_main body_myId.
 semax_func_cons body_main.
-*)
-Abort.
+Qed.
+
+Check prog_correct.
 
